Hoare logic laws and updated parser

UTP/ITree_Procedure.thy
@@ -5,21 +5,31 @@ theory ITree_Procedure
   keywords "over"
 begin
 
+definition "rbind x = (\<lambda> (r, s). Ret (put\<^bsub>x\<^esub> s r))"
+
+definition "rdrop = (\<lambda> (r, s). Ret s)"
+
 definition proc_call :: 
   "('r \<Longrightarrow> 's) \<Rightarrow> ('a \<Rightarrow> 's \<Rightarrow> ('e, 'r \<times> 's) itree) \<Rightarrow> ('a, 's) expr \<Rightarrow> ('e, 's) htree" where
 [code_unfold]: 
-  "proc_call x pr prm = (\<lambda> s. pr (prm s) s \<bind> (\<lambda> (r, s\<^sub>0). Ret (put\<^bsub>x\<^esub> s\<^sub>0 r)))"
+  "proc_call x pr prm = (\<lambda> s. pr (prm s) s \<bind> rbind x)"
 
 definition proc_call_nret :: 
   "('a \<Rightarrow> 's \<Rightarrow> ('e, 'r \<times> 's) itree) \<Rightarrow> ('a, 's) expr \<Rightarrow> ('e, 's) htree" where
   [code_unfold]: 
-  "proc_call_nret pr prm = (\<lambda> s. pr (prm s) s \<bind> (\<lambda> (r, s\<^sub>0). Ret s\<^sub>0))"
+  "proc_call_nret pr prm = (\<lambda> s. pr (prm s) s \<bind> rdrop)"
 
 definition proc_ret :: "('s \<Rightarrow> 'a) \<Rightarrow> 's \<Rightarrow> ('e, 'a \<times> 's) itree" where 
   "proc_ret e = (\<lambda> s. Ret (e s, s))"
 
+lemma ret_rbind: "proc_ret e ;; rbind x = x := e"
+  by (simp add: proc_ret_def rbind_def seq_itree_def kleisli_comp_def assigns_def expr_defs)
+
+lemma ret_drop: "proc_ret e ;; rdrop = Skip"
+  by (simp add: proc_ret_def rdrop_def Skip_def seq_itree_def kleisli_comp_def)
+
 syntax 
-  "_call"      :: "svid \<Rightarrow> id \<Rightarrow> logic \<Rightarrow> logic" ("_ := call _ _" [61, 0, 61] 61)
+  "_call"      :: "svid \<Rightarrow> id \<Rightarrow> logic \<Rightarrow> logic" ("_ := <_ _>" [61, 0, 61] 61)
   "_call_nret" :: "id \<Rightarrow> logic \<Rightarrow> logic" ("call _ _") 
   "_return"    :: "logic \<Rightarrow> logic" ("return")
 
@@ -28,11 +38,17 @@ translations
   "_call x P e" == "CONST proc_call x P (e)\<^sub>e"
   "_call_nret P e" == "CONST proc_call_nret P (e)\<^sub>e"
 
-lemma hl_procedure_call [hoare_safe]: 
-  assumes "\<And> v. H{P \<and> \<guillemotleft>v\<guillemotright> = e} C(v) {Q}"
+lemma hl_proc_call [hoare_safe]: 
+  assumes "\<And> v. H{P \<and> \<guillemotleft>v\<guillemotright> = e} C(v) ;; rbind x {Q}"
+  shows "H{P} x := <C(e)> {Q}"
+  using assms
+  by (auto simp add: hoare_alt_def proc_call_def seq_itree_def kleisli_comp_def)
+
+lemma hl_proc_call_nret [hoare_safe]: 
+  assumes "\<And> v. H{P \<and> \<guillemotleft>v\<guillemotright> = e} C(v) ;; rdrop {Q}"
   shows "H{P} call C(e) {Q}"
   using assms
-  by (auto simp add: hoare_alt_def procedure_call_def)
+  by (auto simp add: hoare_alt_def proc_call_nret_def seq_itree_def kleisli_comp_def)
 
 ML_file \<open>ITree_Procedure.ML\<close>
 
